update

Test/civl/new/tds.bpl
@@ -1,42 +1,84 @@
+type{:datatype} Msg;
+function{:constructor} Request(cid:int):Msg;
+function{:constructor} None():Msg;
+function{:constructor} Task():Msg;
+function{:constructor} Ack(cid:int):Msg;
+
+const unique DEFAULT: int;
+const unique CREATED: int;
+const unique PROCESSED: int;
+const unique FINISHED: int;
+
+var status:[int]int;
+
+procedure AllocTid() returns (id: int);
+
+procedure {:inline} CreateTask(cid: int)
+{
+    assert status[cid] == DEFAULT;
+    status[cid] := CREATED;
+}
+
+procedure {:inline} ProcessTask(cid: int)
+{
+    assert status[cid] == CREATED;
+    status[cid] := PROCESSED;
+}
+
+procedure {:inline} FinishTask(cid: int)
+{
+    assert status[cid] == PROCESSED;
+    status[cid] := FINISHED;
+}
+
+procedure Send(id: int, m: Msg);
+procedure ServerReceive() returns (m: Msg);
+procedure ClientReceive() returns (m: Msg);
+procedure MasterReceive() returns (m: Msg);
+
 procedure main(sid: int, n: int)
 {
     var i: int;
     var m: Msg;
+    var mid: int;
+    var cid: int;
     
+    call mid := AllocTid();
+    async call master(mid, n);
     i := 0;
     while (i < n) {
-        async client(cid);
+    	call cid := AllocTid();
+        async call client(cid, sid, mid);
 	i := i + 1;
     }
-    async master(mid);
-    call server(sid, n);
     i := 0;
     while (i < n) {
-        m := ServerReceive();
-	assert m is Request;
-	CreateTask(m.cid);
-	send m.cid, Task();
+        call m := ServerReceive();
+	assert is#Request(m);
+	call CreateTask(cid#Request(m)); // DEFAULT -> CREATED	
+	call Send(cid#Request(m), Task());
 	i := i + 1;
     }
 }
 
-procedure client(cid: int, mid: int, sid: int)
+procedure client(cid: int, sid: int, mid: int)
 {
     var m: Msg;
-    send sid, Request(cid);
+    call Send(sid, Request(cid));
     call m := ClientReceive();
-    assert m is Task;
-    ProcessTask(cid);
-    send mid, Ack();
+    assert is#Task(m);
+    call ProcessTask(cid); // CREATED -> PROCESSED
+    call Send(mid, Ack(cid));
 }
 
-procedure master(sid: int, n: int) {
+procedure master(mid: int, n: int) {
     var m: Msg;
     var i: int;
     i := 0;
     while (i < n) { 
         call m := MasterReceive();
-	assert m is Ack(cid);
-	FinishTask(m.cid);
+	assert is#Ack(m);
+	call FinishTask(cid#Ack(m)); // PROCESSED -> FINISHED
+	i := i + 1;
     }
 }
